Update Imp examples

lf/Imp.v
@@ -5,7 +5,7 @@ From Coq Require Import Arith.EqNat. Import Nat.
 From Coq Require Import Lia.
 From Coq Require Import Lists.List. Import ListNotations.
 From Coq Require Import Strings.String.
-
+From LF Require Export Maps.
 
 Module AExp.
   (* Abstract syntax *)
@@ -20,7 +20,7 @@ Module AExp.
   | BTrue
   | BFalse
   | BEq (a1 a2 : aexp)
-  | BNeq (a1 a2 : aexp)
+  | BNEq (a1 a2 : aexp)
   | BLe (a1 a2 : aexp)
   | BGt (a1 a2 : aexp)
   | BNot (b : bexp)
@@ -47,7 +47,7 @@ Module AExp.
     | BTrue => true
     | BFalse => false
     | BEq a1 a2 => (aeval a1) =? (aeval a2)
-    | BNeq a1 a2 => negb ((aeval a1) =? (aeval a2))
+    | BNEq a1 a2 => negb ((aeval a1) =? (aeval a2))
     | BLe a1 a2 => (aeval a1) <=? (aeval a2)
     | BGt a1 a2 => negb ((aeval a1) <=? (aeval a2))
     | BNot b => negb (beval b)
@@ -221,7 +221,7 @@ Fixpoint optimize_0plus_b (b : bexp) : bexp :=
   | BTrue => BTrue
   | BFalse => BFalse
   | BEq a1 a2 => BEq (optimize_0plus a1) (optimize_0plus a2)
-  | BNeq a1 a2 => BNeq (optimize_0plus a1) (optimize_0plus a2)
+  | BNEq a1 a2 => BNEq (optimize_0plus a1) (optimize_0plus a2)
   | BLe a1 a2 => BLe (optimize_0plus a1) (optimize_0plus a2)
   | BGt a1 a2 => BGt (optimize_0plus a1) (optimize_0plus a2)
   | BNot b => BNot (optimize_0plus_b b)
@@ -346,4 +346,724 @@ Inductive aevalR : aexp -> nat -> Prop :=
   where "e '==>' n" := (aevalR e n) : type_scope.
 
 
+  Theorem aeval_iff_aevalR :
+    forall a n, (a ==> n) <-> aeval a = n.
+  Proof.
+    intros a n.
+    split.
+    - intros H.
+      induction H; simpl;
+      (try rewrite IHaevalR1; try rewrite IHaevalR2; reflexivity).
+    - intros H.
+      generalize dependent n.
+      induction a; simpl; intros; subst.
+      + apply E_ANum.
+      + apply E_APlus.
+        apply IHa1. reflexivity.
+        apply IHa2. reflexivity.
+      + apply E_AMinus.
+        apply IHa1. reflexivity.
+        apply IHa2. reflexivity.
+      + apply E_AMult.
+        apply IHa1. reflexivity.
+        apply IHa2. reflexivity.
+  Qed.
+  
+  Theorem aeval_iff_aevalR' :
+    forall a n, (a ==> n) <-> aeval a = n.
+  Proof.
+    split.
+    - intros H.
+      induction H; subst; reflexivity.
+    - generalize dependent n.
+      induction a; simpl; intros; subst; constructor;
+      try apply IHa1; try apply IHa2; reflexivity.
+  Qed.
+
+  Reserved Notation "e '==>b' b" (at level 90, left associativity).
+
+  Inductive bevalR : bexp -> bool -> Prop :=
+    | E_BTrue : BTrue ==>b true
+    | E_BFalse : BFalse ==>b false 
+    | E_BEq (a1 a2 : aexp) (n1 n2 : nat) :
+      (a1 ==> n1) -> (a2 ==> n2) ->
+      BEq a1 a2 ==>b (n1 =? n2)
+    | E_BNeq (a1 a2 : aexp) (n1 n2 : nat) :
+      (a1 ==> n1) -> (a2 ==> n2) ->
+      BNEq a1 a2 ==>b negb (n1 =? n2)
+    | E_BLe (a1 a2 : aexp) (n1 n2 : nat) :
+      (a1 ==> n1) -> (a2 ==> n2) ->
+      BLe a1 a2 ==>b (n1 <=? n2)
+    | E_BGt (a1 a2 : aexp) (n1 n2 : nat) :
+      (a1 ==> n1) -> (a2 ==> n2) ->
+      BGt a1 a2 ==>b negb (n1 <=? n2)
+    | E_BNot (e : bexp) (b : bool) :
+      (e ==>b b) ->
+      BNot e ==>b negb b
+    | E_BAnd (e1 e2 : bexp) (b1 b2 : bool) :
+      (e1 ==>b b1) -> (e2 ==>b b2) ->
+      BAnd e1 e2 ==>b andb b1 b2
+    | E_BOr (e1 e2 : bexp) (b1 b2 : bool) :
+      (e1 ==>b b1) -> (e2 ==>b b2) ->
+      BOr e1 e2 ==>b orb b1 b2
+    where "e '==>b' b" := (bevalR e b) : type_scope.
+
+  Lemma beval_iff_bevalR :
+    forall b bv, b ==>b bv <-> beval b = bv.
+  Proof.
+  Admitted.
+
 End AExp.
+
+
+Module aevalR_division.
+  Inductive aexp : Type :=
+  | ANum (n : nat)
+  | APlus (a1 a2 : aexp)
+  | AMinus (a1 a2 : aexp)
+  | AMult (a1 a2 : aexp)
+  | ADiv (a1 a2 : aexp).
+
+  Reserved Notation "e '==>' n"
+    (at level 90, left associativity).
+  
+    Inductive aevalR : aexp -> nat -> Prop :=
+    | E_ANum (n : nat) :
+      (ANum n) ==> n
+    | E_APlus (a1 a2 : aexp) (n1 n2 : nat) :
+      (a1 ==> n1) -> (a2 ==> n2) ->
+      (APlus a1 a2) ==> (n1 + n2)
+    | E_AMinus (a1 a2 : aexp) (n1 n2 : nat) :
+      (a1 ==> n1) -> (a2 ==> n2) ->
+      (AMinus a1 a2) ==> (n1 - n2)
+    | E_AMult (a1 a2 : aexp) (n1 n2 : nat) :
+      (a1 ==> n1) -> (a2 ==> n2) ->
+      (AMult a1 a2) ==> (n1 * n2)
+    | E_ADiv (a1 a2 : aexp) (n1 n2 n3 : nat) :
+      (a1 ==> n1) -> (a2 ==> n2) -> (n2 > 0) ->
+      (mult n2 n3 = n1) ->
+      (ADiv a1 a2) ==> n3
+    where "e '==>' n" := (aevalR e n) : type_scope.
+End aevalR_division.
+
+
+Module aevalR_extended.
+  Reserved Notation "e '==>' n" (at level 90, left associativity).
+
+  Inductive aexp : Type :=
+  | AAny
+  | ANum (n : nat)
+  | APlus (a1 a2 : aexp)
+  | AMinus (a1 a2 : aexp)
+  | AMult (a1 a2 : aexp).
+
+  Inductive aevalR : aexp -> nat -> Prop :=
+  | E_AAny (n : nat) :
+    AAny ==> n
+  | E_ANum (n : nat) :
+    (ANum n) ==> n
+  | E_APlus (a1 a2 : aexp) (n1 n2 : nat) :
+    (a1 ==> n1) -> (a2 ==> n2) -> 
+    (APlus a1 a2) ==> (n1 + n2)
+  | E_AMinus (a1 a2 : aexp) (n1 n2 : nat) :
+    (a1 ==> n1) -> (a2 ==> n2) ->
+    (AMinus a1 a2) ==> (n1 - n2)
+  | E_AMult (a1 a2 : aexp) (n1 n2 : nat) :
+    (a1 ==> n1) -> (a2 ==> n2) ->
+    (AMult a1 a2) ==> (n2 * n2)
+  where "e '==>' n" := (aevalR e n) : type_scope.
+
+
+End aevalR_extended.
+
+Definition state := total_map nat.
+
+
+Inductive aexp : Type :=
+| ANum (n : nat)
+| AId (x : string)
+| APlus (a1 a2 : aexp)
+| AMinus (a1 a2 : aexp)
+| AMult (a1 a2 : aexp).
+
+
+Definition W : string := "W".
+Definition X : string := "X".
+Definition Y : string := "Y".
+Definition Z : string := "Z".
+
+
+Inductive bexp : Type :=
+| BTrue
+| BFalse
+| BEq (a1 a2 : aexp)
+| BNEq (a1 a2 : aexp)
+| BLe (a1 a2 : aexp)
+| BGt (a1 a2 : aexp)
+| BNot (b : bexp)
+| BOr (b1 b2 : bexp)
+| BAnd (b1 b2 : bexp).
+
+
+Coercion AId : string >-> aexp.
+Coercion ANum : nat >-> aexp.
+
+Declare Custom Entry com.
+Declare Scope com_scope.
+
+
+Notation "<{ e }>" :=
+  (e)
+  (at level 0, e custom com at level 99)
+  : com_scope.
+Notation "( x )" :=
+  (x)
+  (in custom com, x at level 99)
+  : com_scope.
+Notation "x" :=
+  (x)
+  (in custom com at level 0, x constr at level 0)
+  : com_scope.
+Notation "f x .. y" :=
+  (.. (f x) .. y)
+  (in custom com at level 0, only parsing,
+   f constr at level 0, x constr at level 9,
+   y constr at level 9)
+  : com_scope.
+Notation "x + y" :=
+  (APlus x y)
+  (in custom com at level 50, left associativity).
+Notation "x - y" :=
+  (AMinus x y)
+  (in custom com at level 50, left associativity).
+Notation "x * y" :=
+  (AMult x y)
+  (in custom com at level 40, left associativity).
+Notation "'true'" :=
+  (true)
+  (at level 1).
+Notation "'false'" :=
+  (false)
+  (at level 1).
+Notation "'true'" :=
+  (BTrue)
+  (in custom com at level 1).
+Notation "'false'" :=
+  (BFalse)
+  (in custom com at level 1).
+Notation "x <= y" :=
+  (BLe x y)
+  (in custom com at level 70, no associativity).
+Notation "x > y" :=
+  (BGt x y)
+  (in custom com at level 70, no associativity).
+Notation "x = y" :=
+  (BEq x y)
+  (in custom com at level 70, no associativity).
+Notation "x <> y" :=
+  (BNEq x y)
+  (in custom com at level 70, no associativity).
+Notation "x '&&' y" :=
+  (BAnd x y)
+  (in custom com at level 80, left associativity).
+Notation "x '||' y" :=
+  (BOr x y)
+  (in custom com at level 80, left associativity).
+Notation "'~' y" :=
+  (BNot y)
+  (in custom com at level 75, right associativity).
+
+Open Scope com_scope.
+
+
+Definition example_aexp : aexp := <{ 3 + (X * 2) }>.
+Definition example_bexp : bexp := <{ true && ~(X <= 4)}>.
+
+Fixpoint aeval (st : state) (a : aexp) : nat :=
+  match a with
+  | ANum n => n
+  | AId x => st x
+  | <{a1 + a2}> => (aeval st a1) + (aeval st a2)
+  | <{a1 - a2}> => (aeval st a1) - (aeval st a2)
+  | <{a1 * a2}> => (aeval st a1) * (aeval st a2)
+  end.
+
+
+Fixpoint beval (st : state) (b : bexp) : bool :=
+  match b with
+  | BTrue => true
+  | BFalse => false
+  | <{ a1 = a2}> => (aeval st a1) =? (aeval st a2)
+  | <{ a1 <> a2}> => negb ((aeval st a1) =? (aeval st a2))
+  | <{ a1 <= a2}> => (aeval st a1) <=? (aeval st a2)
+  | <{ a1 > a2}> => negb ((aeval st a1) <=? (aeval st a2))
+  | <{ ~b }> => negb (beval st b)
+  | <{b1 && b2}> => andb (beval st b1) (beval st b2)
+  | <{b1 || b2}> => orb (beval st b1) (beval st b2)
+  end.
+
+
+Definition empty_st := (_ !-> 0).
+
+
+Notation "x '!->' v" := (x !-> v; empty_st) (at level 100).
+
+
+Example aexp1 :
+  aeval (X !-> 5) <{3 + (X * 2)}> = 13.
+Proof.
+  reflexivity.
+Qed.
+
+
+Example aexp2 :
+    aeval (X !-> 5 ; Y !-> 4) <{ Z + (X * Y) }>
+  = 20.
+Proof.
+  reflexivity.
+Qed.
+
+
+Example bexp1 :
+    beval (X !-> 5) <{ true && ~(X <= 4) }>
+  = true.
+Proof.
+  reflexivity.
+Qed.
+
+
+Inductive com : Type :=
+| CSkip
+| CAsgn (x : string) (a : aexp)
+| CSeq (c1 c2 : com)
+| CIf (b : bexp) (c1 c2 : com)
+| CWhile (b : bexp) (c : com).
+
+
+Notation "'skip'" :=
+  (CSkip)
+  (in custom com at level 0)
+  : com_scope.
+Notation "x ':=' y" :=
+  (CAsgn x y)
+  (in custom com at level 0, x constr at level 0,
+   y at level 85, no associativity)
+  : com_scope.
+Notation "x ';' y" :=
+  (CSeq x y)
+  (in custom com at level 90, right associativity)
+  : com_scope.
+Notation "'if' x 'then' y 'else' z 'end'" :=
+  (CIf x y z)
+  (in custom com at level 89, x at level 99,
+   y at level 99, z at level 99)
+  : com_scope.
+Notation "'while' x 'do' y 'end'" :=
+  (CWhile x y)
+  (in custom com at level 89, x at level 99, y at level 99)
+  : com_scope.
+
+
+Definition fact_in_coq : com :=
+  <{
+    Z := X;
+    Y := 1;
+    while Z <> 0 do
+      Y := Y * Z;
+      Z := Z - 1
+    end
+  }>.
+
+
+Print fact_in_coq.
+
+
+Unset Printing Notations.
+Print fact_in_coq.
+Set Printing Notations.
+
+
+Print example_bexp.
+Set Printing Coercions.
+Print example_bexp.
+Print fact_in_coq.
+Unset Printing Coercions.
+
+
+Locate aexp.
+Locate "&&".
+Locate "||".
+Locate ";".
+Locate "while".
+
+
+Definition plus2 : com :=
+  <{ X := X + 2 }>.
+
+Definition XtimesYinZ : com :=
+  <{ Z := X * Y }>.
+
+Definition substract_slowly_body : com :=
+  <{
+    Z := Z - 1;
+    X := X -1
+  }>.
+
+
+Definition substract_slowly : com :=
+  <{
+    while X <> 0 do
+      substract_slowly_body
+    end
+  }>.
+
+
+Definition substract_3_from_5_slowly : com :=
+  <{
+    X := 3;
+    Z := 5;
+    substract_slowly
+  }>.
+
+
+Definition loop : com :=
+  <{
+    while true do
+      skip
+    end
+  }>.
+
+
+Fixpoint ceval_fun_not_while (st : state) (c : com) : state :=
+  match c with
+  | <{ skip }>
+    => st
+  | <{ x := a }>
+    => (x !-> (aeval st a); st)
+  | <{ c1 ; c2 }>
+    => let st' := ceval_fun_not_while st c1 in
+       ceval_fun_not_while st' c2
+  | <{ if b then c1 else c2 end }>
+    => if (beval st b) then ceval_fun_not_while st c1
+       else ceval_fun_not_while st c2
+  | <{ while b do c end }>
+    => st (* TODO *)
+  end.
+
+
+Reserved Notation "st '=[' c ']=>' st'"
+  (at level 40, c custom com at level 99,
+   st constr, st' constr at next level).
+
+Inductive ceval : com -> state -> state -> Prop :=
+  | E_Skip : forall st, st =[ skip ]=> st
+  | E_Asgn : forall st a n x,
+             aeval st a = n ->
+             st =[ x := a ]=> (x !-> n; st)
+  | E_Seq : forall st st' st'' c1 c2,
+             st =[ c1 ]=> st' ->
+             st' =[ c2 ]=> st'' ->
+             st =[c1 ; c2]=> st''
+  | E_IfTrue : forall st st' b c1 c2,
+             beval st b = true ->
+             st =[ c1 ]=> st' ->
+             st =[if b then c1 else c2 end]=> st'
+  | E_IfFalse : forall st st' b c1 c2,
+             beval st b = false ->
+             st =[ c2 ]=> st' ->
+             st =[if b then c1 else c2 end]=> st'
+  | E_WhileFalse : forall st b c,
+             beval st b = false ->
+             st =[while b do c end]=> st
+  | E_WhileTrue : forall st st' st'' b c,
+             beval st b = true ->
+             st =[ c ]=> st' ->
+             st' =[while b do c end]=> st'' ->
+             st =[while b do c end]=> st''
+  where "st '=[' c ']=>' st'" := (ceval c st st').
+
+
+Example ceval_example1 :
+  empty_st =[
+    X := 2;
+    if (X <= 1) then Y := 3
+    else Z := 4
+    end
+  ]=> (Z !-> 4; X !-> 2).
+Proof.
+  apply E_Seq with (X !-> 2). (* The intermidiate state *)
+  - apply E_Asgn.
+    reflexivity.
+  - apply E_IfFalse.
+    reflexivity.
+    apply E_Asgn.
+    reflexivity.
+Qed.
+
+
+
+Example ceval_example2:
+  empty_st =[
+    X := 0;
+    Y := 1;
+    Z := 2
+  ]=> (Z !-> 2 ; Y !-> 1 ; X !-> 0).
+Proof.
+  apply E_Seq with (X !-> 0).
+  - apply E_Asgn.
+    reflexivity.
+  - apply E_Seq with (Y !-> 1; X !-> 0).
+    + apply E_Asgn.
+      reflexivity.
+    + apply E_Asgn.
+      reflexivity.
+Qed.
+
+
+Set Printing Implicit.
+Check @ceval_example2.
+
+
+Definition pup_to_n : com :=
+  <{
+    Y := 0;
+    while X <> 0 do
+      Y := Y + X;
+      X := X - 1
+    end
+  }>.
+
+
+Theorem pup_to_2_ceval :
+  (X !-> 2) =[
+    pup_to_n
+  ]=> (X !-> 0 ; Y !-> 3 ; X !-> 1 ; Y !-> 2 ; Y !-> 0 ; X !-> 2).
+Proof.
+  unfold pup_to_n.
+  apply E_Seq with (Y !-> 0 ; X !-> 2).
+  - apply E_Asgn.
+    reflexivity.
+  - apply E_WhileTrue with (X !-> 1 ;Y !-> 2; Y !-> 0; X !-> 2).
+    + reflexivity.
+    + apply E_Seq with (Y !-> 2; Y !-> 0; X !-> 2).
+      * apply E_Asgn.
+        reflexivity.
+      * apply E_Asgn.
+        reflexivity.
+    + apply E_WhileTrue with (X !-> 0 ;Y !-> 3 ;X !-> 1 ;Y !-> 2; Y !-> 0; X !-> 2).
+      * reflexivity.
+      * apply E_Seq with (Y !-> 3 ;X !-> 1 ;Y !-> 2; Y !-> 0; X !-> 2).
+        ** apply E_Asgn.
+           reflexivity.
+        ** apply E_Asgn.
+           reflexivity.
+      * apply E_WhileFalse.
+        reflexivity.
+Qed.
+
+
+Theorem ceval_deterministic: forall c st st1 st2,
+     st =[ c ]=> st1 ->
+     st =[ c ]=> st2 ->
+     st1 = st2.
+Proof.
+  intros c st st1 st2 E1 E2.
+  generalize dependent st2.
+  induction E1; intros st2 E2; inversion E2; subst.
+  - reflexivity.
+  - reflexivity.
+  - rewrite (IHE1_1 st'0 H1) in *.
+    apply IHE1_2.
+    assumption.
+  - apply IHE1.
+    assumption.
+  - apply IHE1.
+    rewrite H in H5.
+    discriminate.
+  - apply IHE1.
+    rewrite H in H5.
+    discriminate.
+  - apply IHE1.
+    apply H6.
+  - reflexivity.
+  - rewrite H in H2.
+    discriminate.
+  - rewrite H in H4.
+    discriminate.
+  - rewrite (IHE1_1 st'0 H3) in *.
+    apply IHE1_2.
+    assumption.
+Qed.
+
+
+Theorem plus2_spec : forall st n st',
+  st X = n ->
+  st =[ plus2 ]=> st' ->
+  st' X = n + 2.
+Proof.
+  intros.
+  inversion H0.
+  subst.
+  simpl.
+  apply t_update_eq.
+Qed.
+
+
+Module StackMachine.
+  Inductive sinstr : Type :=
+  | SPush (n : nat)
+  | SLoad (x : string)
+  | SPlus
+  | SMinus
+  | SMult.
+
+
+  Fixpoint s_execute (st : state) (stack : list nat) (prog : list sinstr)
+          : list nat :=
+  match prog with
+  | [] => stack
+  | (SPush n) :: prog' => s_execute st (n :: stack) prog'
+  | (SLoad x) :: prog' => s_execute st ((st x) :: stack) prog'
+  | SPlus :: prog' => 
+    let stack'' := match stack with
+    | [] => []
+    | [a] => [a]
+    | a :: b :: stack' => (a + b) :: stack'
+    end in
+    s_execute st stack'' prog'
+  | SMinus :: prog' =>
+    let stack'' := match stack with
+    | [] => []
+    | [a] => [a]
+    | a :: b :: stack' => (b - a) :: stack'
+    end in
+    s_execute st stack'' prog'
+  | SMult :: prog' => 
+    let stack'' := match stack with
+    | [] => []
+    | [a] => [a]
+    | a :: b :: stack' => (a * b) :: stack'
+    end in
+    s_execute st stack'' prog'
+  end.
+
+
+  Check s_execute.
+
+
+  Example s_execute1 :
+    s_execute empty_st []
+    [SPush 5; SPush 3; SPush 1; SMinus]
+    = [2; 5].
+  Proof.
+    simpl.
+    reflexivity.
+  Qed.
+
+
+  Example s_execute2 :
+    s_execute (X !-> 3) [3;4]
+    [SPush 4; SLoad X; SMult; SPlus]
+    = [15; 4].
+  Proof.
+    simpl.
+    reflexivity.
+  Qed.
+
+  Fixpoint s_compile (e : aexp) : list sinstr :=
+    match e with
+    | ANum n => [SPush n]
+    | AId x => [SLoad x]
+    | <{ a1 + a2}> =>
+      (s_compile a1) ++ (s_compile a2) ++ [SPlus]
+    | <{ a1 - a2 }> =>
+      (s_compile a1) ++ (s_compile a2) ++ [SMinus]
+    | <{ a1 * a2 }> =>
+      (s_compile a1) ++ (s_compile a2) ++ [SMult]
+    end.
+
+  Example s_compile1 :
+    s_compile <{ X - (2 * Y) }>
+    = [SLoad X; SPush 2; SLoad Y; SMult; SMinus].
+  Proof.
+    simpl.
+    reflexivity.
+  Qed.
+
+  Lemma s_compile_correct_aux : forall st e stack,
+    s_execute st stack (s_compile e) = aeval st e :: stack.
+  Proof.
+    intros st e.
+    induction e.
+    - simpl.
+      reflexivity.
+    - simpl.
+      reflexivity.
+    - intros stack.
+      simpl.
+  Admitted.
+
+
+  Theorem s_compile_correct : forall (st : state) (e : aexp),
+    s_execute st [] (s_compile e) = [ aeval st e ].
+  Proof.
+  Admitted.
+
+End StackMachine.
+
+
+Module BreakImp.
+
+  Inductive com : Type :=
+  | CSKip
+  | CBreak
+  | CAsgn (x : string) (a : aexp)
+  | CSeq (c1 c2 : com)
+  | CIf (b : bexp) (c1 c2 : com)
+  | CWhile (b : bexp) (c : com).
+
+  Notation "'break'" :=
+    (CBreak)
+    (in custom com at level 0)
+    : com_scope.
+  Notation "'skip'" :=
+    (CSkip)
+    (in custom com at level 0)
+    : com_scope.
+  Notation "x ':=' y" :=
+    (CAsgn x y)
+    (in custom com at level 0, x constr at level 0,
+     y at level 85, no associativity)
+    : com_scope.
+  Notation "x ; y" :=
+    (CSeq x y)
+    (in custom com at level 90, right associativity)
+    : com_scope.
+  Notation "'if' x 'then' y 'else' z 'end'" :=
+    (CIf x y z)
+    (in custom com at level 89, x at level 99,
+     y at level 99, z at level 99)
+    : com_scope.
+  Notation "'while' x 'do' y 'end'" :=
+    (CWhile x y)
+    (in custom com at level 89,
+     x at level 99, y at level 99)
+    : com_scope.
+  
+  Inductive result : Type :=
+  | SContinue
+  | SBreak.
+  
+  Reserved Notation "st '=[' c ']=>' st' '/' s"
+    (at level 40, c custom com at level 99,
+     st' constr at next level).
+  
+  Inductive ceval : com -> state -> result -> state -> Prop :=
+    | E_Skip : forall st,
+      st =[ CSKip ]=> st / SContinue
+    where "st '=[' c ']=>' st' '/' s" := ceval c st s st'.
+  
+  
+
+End BreakImp.
+
